code/experimental/ed25519/Hacl.Impl.Ed25519.SecretExpand.fst
@@ -18,8 +18,8 @@ let secret_expand expanded secret =
   assert((as_seq h h_low, as_seq h h_high) == Seq.split (as_seq h expanded) 32);
   let h_low0  = h_low.( 0ul) in
   let h_low31 = h_low.(31ul) in
-  h_low.( 0ul) <- (h_low0 &^ 0xf8uy);
-  h_low.(31ul) <- ((h_low31 &^ 127uy) |^ 64uy);
+  h_low.( 0ul) <- (h_low0 &^ Hacl.Cast.uint8_to_sint8 0xf8uy);
+  h_low.(31ul) <- ((h_low31 &^ Hacl.Cast.uint8_to_sint8 127uy) |^ Hacl.Cast.uint8_to_sint8 64uy);
   let h' = ST.get() in
   no_upd_lemma_1 h h' h_low h_high;
   assert( as_seq h' h_high == as_seq h h_high);
