code/experimental/ed25519/Hacl.Impl.Load51.fsti
@@ -9,6 +9,7 @@ open Hacl.Spec.Bignum.Bigint
 open Hacl.Endianness
 open Hacl.UInt64
 
+open Hacl.Spec.Endianness
 
 #reset-options "--max_fuel 0 --z3rlimit 10"
 
@@ -22,5 +23,6 @@ val load_51: output:felem -> input:hint8_p{length input = 32} -> Stack unit
   (ensures (fun h0 _ h1 -> Buffer.live h0 output /\ Buffer.live h0 input
     /\ Buffer.live h1 output /\ modifies_1 output h0 h1
     /\ Hacl.Bignum25519.red_51 (as_seq h1 output)
-    /\ (let out = as_seq h1 output in
-       v (Seq.index out 0) + pow2 51 * v (Seq.index out 1) + pow2 102 * v (Seq.index out 2)  + pow2 153 * v (Seq.index out 3)  + pow2 204 * v (Seq.index out 4) == Endianness.little_endian (as_seq h0 input) % pow2 255)))
+    /\ (let out = reveal_h64s (as_seq h1 output) in
+       let open FStar.UInt64 in
+       v (Seq.index out 0) + pow2 51 * v (Seq.index out 1) + pow2 102 * v (Seq.index out 2)  + pow2 153 * v (Seq.index out 3)  + pow2 204 * v (Seq.index out 4) == hlittle_endian (as_seq h0 input) % pow2 255)))
