code/experimental/ed25519/Hacl.Impl.Load56.fsti
@@ -6,6 +6,7 @@ open FStar.Endianness
 open Hacl.Endianness
 open Hacl.UInt64
 
+open Hacl.Spec.Endianness
 
 #reset-options "--max_fuel 0 --z3rlimit 20"
 
@@ -21,8 +22,9 @@ val load_64_bytes:
   Stack unit
     (requires (fun h -> live h out /\ live h b))
     (ensures (fun h0 _ h1 -> live h1 out /\ modifies_1 out h0 h1 /\ live h0 b
-      /\ (let out = as_seq h1 out in
+      /\ (let out = reveal_h64s (as_seq h1 out) in
          let op_String_Access = Seq.index in
+         let open FStar.UInt64 in
          v out.[0] < 0x100000000000000
          /\ v out.[1] < 0x100000000000000
          /\ v out.[2] < 0x100000000000000
@@ -33,9 +35,9 @@ val load_64_bytes:
          /\ v out.[7] < 0x100000000000000
          /\ v out.[8] < 0x100000000000000
          /\ v out.[9] < 0x100000000000000
-         /\ little_endian (as_seq h0 b)
+         /\ little_endian (reveal_sbytes (as_seq h0 b))
           == Hacl.Spec.BignumQ.Eval.eval_q_10 out.[0] out.[1] out.[2] out.[3] out.[4] out.[5] out.[6] out.[7] out.[8] out.[9]
-        /\ little_endian (as_seq h0 b) < pow2 512)
+        /\ little_endian (reveal_sbytes (as_seq h0 b)) < pow2 512)
     ))
 
 
@@ -45,12 +47,13 @@ val load_32_bytes:
   Stack unit
     (requires (fun h -> live h out /\ live h b))
     (ensures (fun h0 _ h1 -> live h1 out /\ modifies_1 out h0 h1 /\ live h0 b
-      /\ (let out = as_seq h1 out in
+      /\ (let out = reveal_h64s (as_seq h1 out) in
          let op_String_Access = Seq.index in
+         let open FStar.UInt64 in
          v out.[0] < 0x100000000000000
          /\ v out.[1] < 0x100000000000000
          /\ v out.[2] < 0x100000000000000
          /\ v out.[3] < 0x100000000000000
          /\ v out.[4] < 0x100000000000000 /\
-         little_endian (as_seq h0 b)
+         little_endian (reveal_sbytes (as_seq h0 b))
           == Hacl.Spec.BignumQ.Eval.eval_q out)))
