code/experimental/ed25519/Hacl.Impl.SHA512.ModQ.fsti
@@ -3,6 +3,7 @@ module Hacl.Impl.SHA512.ModQ
 open FStar.Buffer
 open Hacl.UInt64
 
+open Hacl.Spec.Endianness
 
 #reset-options "--max_fuel 0 --z3rlimit 20"
 
@@ -15,7 +16,7 @@ val sha512_modq_pre:
         (requires (fun h0 -> live h0 input /\ live h0 out /\ live h0 prefix))
         (ensures  (fun h0 _ h1 -> live h0 input /\ live h1 out /\ modifies_1 out h0 h1 /\
           live h0 prefix /\ live h1 prefix /\
-          Hacl.Spec.BignumQ.Eval.eval_q (as_seq h1 out) == Spec.Ed25519.sha512_modq FStar.Seq.(as_seq h0 prefix @| as_seq h0 input) /\
+          Hacl.Spec.BignumQ.Eval.eval_q (reveal_h64s (as_seq h1 out)) == Spec.Ed25519.sha512_modq FStar.Seq.(reveal_sbytes (as_seq h0 prefix @| as_seq h0 input)) /\
           (let out = as_seq h1 out in let op_String_Access = Seq.index in
            v (out.[0]) < 0x100000000000000 /\ v (out.[1]) < 0x100000000000000 /\
            v (out.[2]) < 0x100000000000000 /\ v (out.[3]) < 0x100000000000000 /\
@@ -31,7 +32,7 @@ val sha512_modq_pre_pre2:
         (requires (fun h -> live h input /\ live h out /\ live h prefix /\ live h prefix2))
         (ensures  (fun h0 _ h1 -> live h0 input /\ live h1 out /\ modifies_1 out h0 h1 /\
           live h0 prefix /\ live h1 prefix /\ live h0 prefix2 /\ live h1 prefix2 /\
-          Hacl.Spec.BignumQ.Eval.eval_q (as_seq h1 out) == Spec.Ed25519.sha512_modq FStar.Seq.(as_seq h0 prefix @| as_seq h0 prefix2 @| as_seq h0 input) /\
+          Hacl.Spec.BignumQ.Eval.eval_q (reveal_h64s (as_seq h1 out)) == Spec.Ed25519.sha512_modq FStar.Seq.(reveal_sbytes (as_seq h0 prefix @| as_seq h0 prefix2 @| as_seq h0 input)) /\
           (let out = as_seq h1 out in let op_String_Access = Seq.index in
            v (out.[0]) < 0x100000000000000 /\ v (out.[1]) < 0x100000000000000 /\
            v (out.[2]) < 0x100000000000000 /\ v (out.[3]) < 0x100000000000000 /\
